\documentclass{article}

\usepackage{amsfonts}
\usepackage{amsmath}
\usepackage{graphicx}
\usepackage{float}
\usepackage{caption}
\usepackage{subcaption}

\renewcommand\thesubsection{\alph{subsection})}

\title{\textbf{Assignment 3}}
\author{Anna Pavlova}
\date{April 2016}

\begin{document}

\maketitle

\section{}
$$\mathrm{KL}(p||q)=\mathbb{E}_p\log\frac{p}{q} = \mathbb{E}_p\log p - \mathbb{E}_p \log q = -\mathbb{H}p - \sum_{i=1}^N\mathbb{E}_{p(\mathbf{Z}_i)}\log q(\mathbf{Z}_i) = $$ $$= -\mathbb{H}p(\mathbf{Z}) - \sum_{i=1}^N\mathbb{H}p(\mathbf{Z}_i) + \sum_{i=1}^N\mathrm{KL}(p(\mathbf{Z}_i)||q(\mathbf{Z}_i))$$
From this identity we obtain that:
$$q^{*}(\mathbf{Z}_i) = p(\mathbf{Z}_i) = \int p(\mathbf{Z})\prod_{j \neq i}d\mathbf{Z}_j$$
However, according to the problem, the technique of Lagrange multipliers should be used, so let us find minimum of $\mathrm{KL}(p||q)$ using the approach (it will be equal to the initial problem statement):
$$\delta \Big[ \mathrm{KL}(p||q) - \lambda \Big(\int q(\mathbf{Z}) d\mathbf{Z} - 1\Big) \Big] = -\int \frac{p(\mathbf{Z})}{q(\mathbf{Z})} \delta q(\mathbf{Z})d\mathbf{Z} - \lambda \int \delta q(\mathbf{Z})d\mathbf{Z} = $$
$$= -\int \Big(\frac{p(\mathbf{Z})}{q(\mathbf{Z})} + \lambda\Big) \delta q(\mathbf{Z})d\mathbf{Z} = 0$$
$$q(\mathbf{Z}) = -\frac{1}{\lambda}q(\mathbf{Z})$$

We see that $q(\mathbf{Z}) \propto p(\mathbf{Z})$ and using the fact that both $p$ and $q$ are distributions we conclude that $p = q$.

\section{}
Let us derive the ELBO:
$$\mathcal{L}(q) = \mathbb{E}_{q(\mathbf{Z})q(\pmb{\theta})} \log \frac{p(\mathbf{Z}, \pmb{\theta})}{q(\mathbf{Z})q(\mathbf{\theta})} = \mathbb{E}_{q(\mathbf{Z})} \log \frac{p(\mathbf{Z}, \mathbf{\pmb\theta_0})}{q(\mathbf{Z})} + \mathbb{H}q(\pmb\theta)$$
$\mathbb{H}q(\pmb\theta)$ is infinite but constant, because entropy does not depend on shift $\pmb\theta_0$. So we can define a new function:
$$\mathcal{\tilde{L}}(q, \pmb\theta_0) = \mathbb{E}_{q(\mathbf{Z})} \log \frac{p(\mathbf{Z}, \mathbf{\pmb\theta_0})}{q(\mathbf{Z})} = \mathcal{L}(q) + \mathrm{const}$$
According to deriving of EM algorithm, optimizing it by $q(\pmb z)$ is equivalent to E-step, by $\pmb\theta_0$ to M-step.  
\end{document}
